-- Generic conversion between stores and memory

open import Lattice

module Generic.Store.Convert
  {{ğ‘³ : Lattice}}
  {Tyâ‚ Tyâ‚‚ : Set}
  {Valueâ‚ : Tyâ‚ â†’ Set}
  {Valueâ‚‚ : Tyâ‚‚ â†’ Set}
  (âŸª_âŸ«áµ— : Tyâ‚ â†’ Tyâ‚‚)
  (âŸª_âŸ«â±½ : âˆ€ {Ï„} â†’ Valueâ‚ Ï„ â†’ Label â†’ Valueâ‚‚ âŸª Ï„ âŸ«áµ—) where

open import Generic.Store.Base as B using ([] ; _âˆ·_)

module S = B Tyâ‚ Valueâ‚
module T = B Tyâ‚‚ Valueâ‚‚

-- Generic pointwise memory transformation
âŸª_âŸ«á´¹ : âˆ€ {â„“} â†’ S.Memory â„“ â†’ T.Memory â„“
âŸª_âŸ«á´¹ [] = []
âŸª_âŸ«á´¹ {â„“} (v âˆ· M) = âŸª v âŸ«â±½ â„“ âˆ· âŸª M âŸ«á´¹

-- Generic pointwise store transformation
âŸª_âŸ«Ë¢ : S.Store â†’ T.Store
âŸª Î£ âŸ«Ë¢ â„“ = âŸª Î£ â„“ âŸ«á´¹

infix 2 âŸª_âŸ«Ë¢

module Lemmas where

  open import Relation.Binary.PropositionalEquality
  open import Relation.Nullary

  âˆ¥_âˆ¥-â‰¡á´¹ : âˆ€ {â„“} (M : S.Memory â„“) â†’ T.âˆ¥ âŸª M âŸ«á´¹ âˆ¥ â‰¡ S.âˆ¥ M âˆ¥
  âˆ¥ [] âˆ¥-â‰¡á´¹ = refl
  âˆ¥ v âˆ· M âˆ¥-â‰¡á´¹ rewrite âˆ¥ M âˆ¥-â‰¡á´¹ = refl

  âˆ¥_âˆ¥-â‰¡ : âˆ€ Î£ â„“ â†’ T.âˆ¥ âŸª Î£ âŸ«Ë¢ â„“ âˆ¥ â‰¡ S.âˆ¥ Î£ â„“ âˆ¥
  âˆ¥_âˆ¥-â‰¡ Î£ â„“ = âˆ¥ (Î£ â„“) âˆ¥-â‰¡á´¹

  âˆ·á´¿-â‰¡ : âˆ€ {â„“ Ï„} (v : Valueâ‚ Ï„) (M : S.Memory â„“) â†’ âŸª M âŸ«á´¹ T.âˆ·á´¿ âŸª v âŸ«â±½ â„“ â‰¡ âŸª M S.âˆ·á´¿ v âŸ«á´¹
  âˆ·á´¿-â‰¡ v [] = refl
  âˆ·á´¿-â‰¡ v (_ âˆ· M) = congâ‚‚ _âˆ·_ refl (âˆ·á´¿-â‰¡ v M)

  update-â‰¡Ë¢ : âˆ€ {â„“ Î£ Mâ‚ Mâ‚‚} â†’ Mâ‚ â‰¡ âŸª Mâ‚‚ âŸ«á´¹ â†’ (â„“' : Label) â†’
              ((âŸª Î£ âŸ«Ë¢ T.[ â„“ â†¦ Mâ‚ ]Ë¢) â„“' â‰¡ âŸª Î£ S.[ â„“ â†¦ Mâ‚‚ ]Ë¢ âŸ«Ë¢ â„“')
  update-â‰¡Ë¢ {â„“} eq â„“' with â„“ â‰Ÿ â„“'
  ... | yes refl = eq
  ... | no Â¬p = refl

  âŸª_âŸ«âˆˆá´¹ : âˆ€ {â„“ Ï„ n} {v : Valueâ‚ Ï„} {M : S.Memory â„“} â†’ n S.â†¦ v âˆˆá´¹ M â†’ n T.â†¦ (âŸª v âŸ«â±½ â„“) âˆˆá´¹ âŸª M âŸ«á´¹
  âŸª S.Here âŸ«âˆˆá´¹ = T.Here
  âŸª S.There x âŸ«âˆˆá´¹ = T.There âŸª x âŸ«âˆˆá´¹

  write-â‰¡á´¹ : âˆ€ {â„“ n Ï„} {M M' : S.Memory â„“} {v : Valueâ‚ Ï„} â†’ M' S.â‰” M [ n â†¦ v ]á´¹ â†’ âŸª M' âŸ«á´¹ T.â‰” âŸª M âŸ«á´¹ [ n â†¦ (âŸª v âŸ«â±½ â„“) ]á´¹
  write-â‰¡á´¹ S.Here = T.Here
  write-â‰¡á´¹ (S.There x) = T.There (write-â‰¡á´¹ x)

------------------------------------------------------------------------------------------
