module FG2CG.Graph.Types  where

open import FG.Types as FG
open import CG.Types as CG
open import FG2CG.Types
open import Relation.Binary.PropositionalEquality

mutual

  data MkTyâ€² : FG.Ty â†’ CG.Ty â†’ Set where
    ğ“› : MkTyâ€² ğ“› ğ“›
    Unit : MkTyâ€² unit unit
    Refá´µ : âˆ€ {Ï„ Ï„'} â†’ MkTyâ€² Ï„ Ï„' â†’ MkTyâ€² (Ref I Ï„) (Ref I Ï„')
    RefË¢ : âˆ€ {Ï„ Ï„'} â†’ MkTyâ€² Ï„ Ï„' â†’ MkTyâ€² (Ref S Ï„) (Ref S Ï„')
    Sum : âˆ€ {Ï„â‚ Ï„â‚‚ Ï„â‚' Ï„â‚‚'} â†’ MkTy Ï„â‚ Ï„â‚' â†’ MkTy Ï„â‚‚ Ï„â‚‚' â†’ MkTyâ€² (Ï„â‚ FG.+ Ï„â‚‚) (Ï„â‚' CG.+ Ï„â‚‚')
    Prod : âˆ€ {Ï„â‚ Ï„â‚‚ Ï„â‚' Ï„â‚‚'} â†’ MkTy Ï„â‚ Ï„â‚' â†’ MkTy Ï„â‚‚ Ï„â‚‚' â†’ MkTyâ€² (Ï„â‚ FG.Ã— Ï„â‚‚) (Ï„â‚' CG.Ã— Ï„â‚‚')
    Fun : âˆ€ {Ï„â‚ Ï„â‚‚ Ï„â‚' Ï„â‚‚'} â†’ MkTy Ï„â‚ Ï„â‚' â†’ MkTy Ï„â‚‚ Ï„â‚‚' â†’ MkTyâ€² (Ï„â‚ FG.â” Ï„â‚‚) (Ï„â‚' CG.â” (LIO Ï„â‚‚'))
    Id : âˆ€ {Ï„ Ï„'} â†’ MkTy Ï„ Ï„' â†’ MkTyâ€² (Id Ï„) Ï„'

  data MkTy (Ï„ : FG.Ty) : CG.Ty â†’ Set where
    Labeled : âˆ€ {Ï„'} â†’ MkTyâ€² Ï„ Ï„' â†’ MkTy Ï„ (Labeled Ï„')

Boolâ€² : MkTyâ€² FG.Bool âŸª FG.Bool âŸ«áµ—â€²
Boolâ€² = Sum (Labeled Unit) (Labeled Unit)

mutual
  mkTyâ€² : âˆ€ Ï„ â†’ MkTyâ€² Ï„ âŸª Ï„ âŸ«áµ—â€²
  mkTyâ€² unit = Unit
  mkTyâ€² (Ï„ Ã— Ï„â‚) = Prod (mkTy Ï„) (mkTy Ï„â‚)
  mkTyâ€² (Ï„ + Ï„â‚) = Sum (mkTy Ï„) (mkTy Ï„â‚)
  mkTyâ€² (Ï„ â” Ï„â‚) = Fun (mkTy Ï„) (mkTy Ï„â‚)
  mkTyâ€² ğ“› = ğ“›
  mkTyâ€² (Ref I Ï„) = Refá´µ (mkTyâ€² Ï„)
  mkTyâ€² (Ref S Ï„) = RefË¢ (mkTyâ€² Ï„)
  mkTyâ€² (Id Ï„) = Id (mkTy Ï„)

  mkTy : âˆ€ Ï„ â†’ MkTy Ï„ âŸª Ï„ âŸ«áµ—
  mkTy x = Labeled (mkTyâ€² x)

mutual
  â‰¡-MkTy : âˆ€ {Ï„ Ï„'} â†’ MkTy Ï„ Ï„' â†’ Ï„' â‰¡ âŸª Ï„ âŸ«áµ—
  â‰¡-MkTy (Labeled x) = cong Labeled (â‰¡-MkTyâ€² x)

  â‰¡-MkTyâ€² : âˆ€ {Ï„ Ï„'} â†’ MkTyâ€² Ï„ Ï„' â†’ Ï„' â‰¡ âŸª Ï„ âŸ«áµ—â€²
  â‰¡-MkTyâ€² ğ“› = refl
  â‰¡-MkTyâ€² Unit = refl
  â‰¡-MkTyâ€² (Refá´µ x) = cong (Ref I) (â‰¡-MkTyâ€² x)
  â‰¡-MkTyâ€² (RefË¢ x) = cong (Ref S) (â‰¡-MkTyâ€² x)
  â‰¡-MkTyâ€² (Sum x xâ‚) = congâ‚‚ _+_ (â‰¡-MkTy x) (â‰¡-MkTy xâ‚)
  â‰¡-MkTyâ€² (Prod x xâ‚) = congâ‚‚ CG._Ã—_ (â‰¡-MkTy x) (â‰¡-MkTy xâ‚)
  â‰¡-MkTyâ€² (Fun x xâ‚) = congâ‚‚ _â”_ (â‰¡-MkTy x) (cong LIO (â‰¡-MkTy xâ‚))
  â‰¡-MkTyâ€² (Id x) rewrite â‰¡-MkTy x = refl

open import Function.Equivalence

-- The relation MkTy is an equivalent representation for the
-- translation function over types.
MkTy-âŸªÂ·âŸ«áµ— : âˆ€ {Ï„ Ï„'} â†’ Ï„' â‰¡ âŸª Ï„ âŸ«áµ—  â‡”  MkTy Ï„ Ï„'
MkTy-âŸªÂ·âŸ«áµ— = equivalence (Î» { refl â†’ mkTy _ }) â‰¡-MkTy

MkTyâ€²-âŸªÂ·âŸ«áµ—â€² : âˆ€ {Ï„ Ï„'} â†’ Ï„' â‰¡ âŸª Ï„ âŸ«áµ—â€²  â‡”  MkTyâ€² Ï„ Ï„'
MkTyâ€²-âŸªÂ·âŸ«áµ—â€² = equivalence (Î» { refl â†’ mkTyâ€² _ }) â‰¡-MkTyâ€²

mutual

  -- Unique proofs
  !-MkTy : âˆ€ {Ï„ Ï„'} (x y : MkTy Ï„ Ï„') â†’ x â‰¡ y
  !-MkTy (Labeled x) (Labeled y) rewrite !-MkTyâ€² x y = refl

  !-MkTyâ€² : âˆ€ {Ï„ Ï„'} (x y : MkTyâ€² Ï„ Ï„') â†’ x â‰¡ y
  !-MkTyâ€² ğ“› ğ“› = refl
  !-MkTyâ€² Unit Unit = refl
  !-MkTyâ€² (Refá´µ x) (Refá´µ y)
    rewrite !-MkTyâ€² x y = refl
  !-MkTyâ€² (RefË¢ x) (RefË¢ y)
    rewrite !-MkTyâ€² x y = refl
  !-MkTyâ€² (Sum xâ‚ xâ‚‚) (Sum yâ‚ yâ‚‚)
    rewrite !-MkTy xâ‚ yâ‚ | !-MkTy xâ‚‚ yâ‚‚ = refl
  !-MkTyâ€² (Prod xâ‚ xâ‚‚) (Prod yâ‚ yâ‚‚)
    rewrite !-MkTy xâ‚ yâ‚ | !-MkTy xâ‚‚ yâ‚‚ = refl
  !-MkTyâ€² (Fun xâ‚ xâ‚‚) (Fun yâ‚ yâ‚‚)
    rewrite !-MkTy xâ‚ yâ‚ | !-MkTy xâ‚‚ yâ‚‚ = refl
  !-MkTyâ€² (Id x) (Id y)
    rewrite !-MkTy x y = refl

--------------------------------------------------------------------------------

-- Graph instances

open import Generic.Graph

Graph-âŸªÂ·âŸ«áµ— : Graph âŸª_âŸ«áµ—
Graph-âŸªÂ·âŸ«áµ— = record { P = MkTy ; âŒœ_âŒ = mkTy ; âŒ_âŒŸ = â‰¡-MkTy }

Graph-âŸªÂ·âŸ«áµ—â€² : Graph âŸª_âŸ«áµ—â€²
Graph-âŸªÂ·âŸ«áµ—â€² = record { P = MkTyâ€² ; âŒœ_âŒ = mkTyâ€² ; âŒ_âŒŸ = â‰¡-MkTyâ€² }

-- Derive graph of context generically.
open import Generic.Context.Graph {FG.Ty} {CG.Ty} {âŸª_âŸ«áµ—} Graph-âŸªÂ·âŸ«áµ—
  renaming ( S2Tá¶œ to MkCtx
           ; mkS2Tá¶œ to mkCtx
           ; â‰¡-S2Tá¶œ to â‰¡-MkCtx
           ; S2T-âˆˆ to Fg2Cg-âˆˆ
           ; mkS2T-âˆˆ to mkFg2Cg-âˆˆ
           ; â‰¡-S2T-âˆˆ to â‰¡-Fg2Cg-âˆˆ
           ; S2T-âŠ† to Fg2Cg-âŠ†
           ; mkS2T-âŠ† to mkFg2Cg-âŠ†
           ; â‰¡-S2T-âŠ† to â‰¡-Fg2Cg-âŠ† ) public

-- Derive uniqueness proof generically.
open Unique !-MkTy renaming (!-S2Tá¶œ to !-MkCtx) public
